word_lang updated with Inst and Get commands

new-backend/word_langScript.sml
@@ -1,9 +1,9 @@
-open HolKernel Parse boolLib bossLib; 
+open HolKernel Parse boolLib bossLib;
 val _ = new_theory "word_lang";
 
 open pred_setTheory arithmeticTheory pairTheory listTheory combinTheory;
 open finite_mapTheory sumTheory relationTheory stringTheory optionTheory;
-open wordsTheory sptreeTheory lcsymtacs bvpTheory;
+open wordsTheory sptreeTheory lcsymtacs bvpTheory asmTheory;
 
 infix \\ val op \\ = op THEN;
 
@@ -24,26 +24,22 @@ val _ = Datatype `
           | WordWidth ('a word)`
 
 val _ = Datatype `
-  word_op = AND | ADD | OR | SUB | MUL | XOR`
-
-val _ = Datatype `
-  word_sh = LSL | LSR | ASR`
-
-val _ = Datatype `
   word_exp = Const ('a word)
            | Var num
-           | Get store_name
+           | Lookup store_name
            | Load word_exp
-           | Op word_op (word_exp list)
-           | Shift word_sh word_exp ('a num_exp)`
+           | Op binop (word_exp list)
+           | Shift shift word_exp ('a num_exp)`
 
 val _ = Datatype `
   word_prog = Skip
             | Move ((num # num) list)
+            | Inst ('a inst)
             | Assign num ('a word_exp)
+            | Get num store_name
             | Set store_name ('a word_exp)
             | Store ('a word_exp) num
-            | Call ((num # num_set # word_prog) option) 
+            | Call ((num # num_set # word_prog) option)
                    (* return var, cut-set, return-handler code *)
                    (num option) (* target of call *)
                    (num list) (* arguments *)
@@ -123,21 +119,20 @@ val mem_load_def = Define `
 val word_op_def = Define `
   word_op op (ws:('a word) list) =
     case (op,ws) of
-    | (AND,ws) => SOME (FOLDR word_and (~0w) ws)
-    | (ADD,ws) => SOME (FOLDR word_add 0w ws)
-    | (OR,ws) => SOME (FOLDR word_or 0w ws)
-    | (XOR,ws) => SOME (FOLDR word_xor 0w ws)
-    | (SUB,[w1;w2]) => SOME (w1 - w2)
-    | (MUL,[w1;w2]) => SOME (w1 * w2)
+    | (And,ws) => SOME (FOLDR word_and (~0w) ws)
+    | (Add,ws) => SOME (FOLDR word_add 0w ws)
+    | (Or,ws) => SOME (FOLDR word_or 0w ws)
+    | (Xor,ws) => SOME (FOLDR word_xor 0w ws)
+    | (Sub,[w1;w2]) => SOME (w1 - w2)
     | _ => NONE`;
 
 val word_sh_def = Define `
   word_sh sh (w:'a word) n =
     if n <> 0 /\ n < dimindex (:'a) then NONE else
       case sh of
-      | LSL => SOME (w << n)
-      | LSR => SOME (w >>> n)
-      | ASR => SOME (w >> n)`;
+      | Lsl => SOME (w << n)
+      | Lsr => SOME (w >>> n)
+      | Asr => SOME (w >> n)`;
 
 val MEM_IMP_word_exp_size = store_thm("MEM_IMP_word_exp_size",
   ``!xs a. MEM a xs ==> (word_exp_size l a < word_exp1_size l xs)``,
@@ -151,7 +146,7 @@ val word_exp_def = tDefine "word_exp" `
      case lookup v s.locals of
      | SOME (Word w) => SOME w
      | _ => NONE) /\
-  (word_exp s (Get name) =
+  (word_exp s (Lookup name) =
      case FLOOKUP s.store name of
      | SOME (Word w) => SOME w
      | _ => NONE) /\
@@ -256,18 +251,18 @@ val list_rearrange_def = Define `
     else (* if it isn't well-formed, just pretend it is I *)
       xs`
 
-(*Compare on keys, if keys match (never), then compare on the word_loc vals
-Treat Words as < Locs*)
+(* Compare on keys, if keys match (never), then compare on
+   the word_loc vals. Treat Words as < Locs *)
 val key_val_compare_def = Define `
   key_val_compare x y =
     let (a:num,b) = x in
     let (a':num,b') = y in
       (a < a') \/
       (a = a' /\
-        case b of 
+        case b of
           Word x => (case b' of Word y => x <= y | _ => T)
         | Loc a b => case b' of Loc a' b' => (a<a') \/ (a=a' /\ b<=b') | _ => F)`
-  
+
 (*
 EVAL ``key_val_compare (1,Loc 3 4) (1,Loc 1 2)``
 *)
@@ -414,6 +409,35 @@ val wAlloc_def = Define `
             | SOME F => (* fail, GC didn't free up enough space *)
                         (SOME NotEnoughSpace,call_env [] s with stack:= [])))))`
 
+val word_assign_def = Define `
+  word_assign reg exp s =
+    case word_exp s exp of
+     | NONE => NONE
+     | SOME w => SOME (set_var reg (Word w) s)`;
+
+val wInst_def = Define `
+  wInst i s =
+    case i of
+    | Skip => NONE
+    | Const reg w => word_assign reg (Const w) s
+    | Arith (Binop bop r1 r2 ri) =>
+        word_assign r1
+          (Op bop [Var r2; case ri of Reg r3 => Var r2
+                                    | Imm w => Const w]) s
+    | Arith (Shift shift r1 r2 n) =>
+        word_assign r1
+          (Shift shift (Var r2) (Nat n)) s
+    | Mem Load r (Addr a w) =>
+        word_assign r (Load (Op Add [Var a; Const w])) s
+    | Mem Store r (Addr q w) =>
+       (case (word_exp s (Op Add [Var a; Const w]), get_var r s) of
+        | (SOME a, SOME w) =>
+            (case mem_store a w s of
+             | SOME s1 => SOME s1
+             | NONE => NONE)
+        | _ => NONE)
+    | _ => NONE`
+
 val wEval_def = tDefine "wEval" `
   (wEval (Skip:'a word_prog,s) = (NONE,s:'a word_state)) /\
   (wEval (Alloc n names,s) =
@@ -426,18 +450,26 @@ val wEval_def = tDefine "wEval" `
        | NONE => (SOME Error,s)
        | SOME vs => (NONE, set_vars (MAP FST moves) vs s)
      else (SOME Error,s)) /\
+  (wEval (Inst i,s) =
+     case wInst i s of
+     | SOME s1 => (NONE, s1)
+     | NONE => (SOME Error, s)) /\
   (wEval (Assign v exp,s) =
      case word_exp s exp of
      | NONE => (SOME Error, s)
      | SOME w => (NONE, set_var v (Word w) s)) /\
+  (wEval (Get v name,s) =
+     case FLOOKUP s.store name of
+     | NONE => (SOME Error, s)
+     | SOME x => (NONE, set_var v x s)) /\
   (wEval (Set v exp,s) =
      case word_exp s exp of
      | NONE => (SOME Error, s)
      | SOME w => (NONE, set_store v (Word w) s)) /\
   (wEval (Store exp v,s) =
      case (word_exp s exp, get_var v s) of
-     | (SOME addr, SOME w) =>
-         (case mem_store addr w s of
+     | (SOME a, SOME w) =>
+         (case mem_store a w s of
           | SOME s1 => (NONE, s1)
           | NONE => (SOME Error, s))
      | _ => (SOME Error, s)) /\
@@ -494,7 +526,7 @@ val wEval_def = tDefine "wEval" `
 		    | NONE => (SOME Error,s2)
 		    | SOME s1 =>
 			(if domain s1.locals = domain env
-			 then 
+			 then
 			   (*Value restriction on the return handler (makes it easier to reason about)
 			     Don't really need it to do fancy things.*)
 			   case wEval(ret_handler,set_var n x (check_clock s1 s)) of
@@ -537,24 +569,31 @@ val wAlloc_clock = store_thm("wAlloc_clock",
   \\ REPEAT BasicProvers.FULL_CASE_TAC \\ SRW_TAC [] [] \\ fs []
   \\ REPEAT BasicProvers.FULL_CASE_TAC \\ SRW_TAC [] [] \\ fs []
   \\ Q.ABBREV_TAC `s3 = set_store AllocSize (Word x) s1`
-  \\ `s3.clock=s1.clock` by Q.UNABBREV_TAC`s3`>>fs[set_store_def] 
+  \\ `s3.clock=s1.clock` by Q.UNABBREV_TAC`s3`>>fs[set_store_def]
   \\ REPEAT BasicProvers.FULL_CASE_TAC \\ SRW_TAC [] [] \\ fs []
-  >- (IMP_RES_TAC wGC_clock 
-     \\ ASSUME_TAC (INST_TYPE [``:'a``|->``:'b``] 
-        (Q.GENL [`env`,`b`,`s`] push_env_clock)) 
+  >- (IMP_RES_TAC wGC_clock
+     \\ ASSUME_TAC (INST_TYPE [``:'a``|->``:'b``]
+        (Q.GENL [`env`,`b`,`s`] push_env_clock))
      \\ first_x_assum(qspecl_then [`s3`,`F`,`x'`] assume_tac)\\fs[]\\rfs[])
   \\ REPEAT BasicProvers.FULL_CASE_TAC \\ SRW_TAC [] [] \\ fs []
   \\ POP_ASSUM MP_TAC \\ SRW_TAC [] []
   \\ IMP_RES_TAC pop_env_clock \\ IMP_RES_TAC wGC_clock
   \\ fs [push_env_clock,set_store_def] \\ SRW_TAC [] []
   \\ Cases_on `env_to_list s1.locals s1.permute` \\ fs [LET_DEF]\\rfs[]
-  \\ BasicProvers.EVERY_CASE_TAC 
+  \\ BasicProvers.EVERY_CASE_TAC
   \\ fs[call_env_def,fetch "-" "word_state_component_equality"]);
 
 val pop_env_clock = prove(
   ``(pop_env s = SOME t) ==> (s.clock = t.clock)``,
   fs [pop_env_def] \\ REPEAT BasicProvers.FULL_CASE_TAC
   \\ SRW_TAC [] [] \\ fs []);
+
+val wInst_clock = prove(
+  ``wInst i s = SOME s2 ==> s2.clock <= s.clock``,
+  Cases_on `i` \\ fs [wInst_def,word_assign_def]
+  \\ REPEAT BasicProvers.FULL_CASE_TAC
+  \\ SRW_TAC [] [set_var_def] \\ fs []
+  \\ fs [mem_store_def] \\ SRW_TAC [] []);
 
 val wEval_clock = store_thm("wEval_clock",
   ``!xs s1 vs s2. (wEval (xs,s1) = (vs,s2)) ==> s2.clock <= s1.clock``,
@@ -563,6 +602,7 @@ val wEval_clock = store_thm("wEval_clock",
   \\ FULL_SIMP_TAC std_ss [cut_state_opt_def]
   \\ REPEAT BasicProvers.FULL_CASE_TAC
   \\ REPEAT STRIP_TAC \\ SRW_TAC [] [check_clock_def,call_env_def]
+  \\ IMP_RES_TAC wInst_clock
   \\ fs [call_env_def]
   \\ RES_TAC \\ IMP_RES_TAC check_clock_IMP
   \\ FULL_SIMP_TAC std_ss [PULL_FORALL] \\ RES_TAC
@@ -621,7 +661,7 @@ val wEval_ind = save_thm("wEval_ind",let
            \\ TRY (`s1.clock <= s.clock` by
              (fs [call_env_def,dec_clock_def,push_env_clock]
              \\ IMP_RES_TAC pop_env_clock \\ DECIDE_TAC)
-           \\ `s1 = check_clock s1 s` by fs[check_clock_def]) 
+           \\ `s1 = check_clock s1 s` by fs[check_clock_def])
            \\ POP_ASSUM (fn th => ONCE_REWRITE_TAC [th])
            \\ FIRST_X_ASSUM MATCH_MP_TAC \\ fs [])
     \\ FIRST_X_ASSUM (MATCH_MP_TAC)
@@ -659,16 +699,14 @@ val wEval_def = save_thm("wEval_def",let
     \\ SRW_TAC [] []
     \\ IMP_RES_TAC wEval_clock
     \\ fs [call_env_def,dec_clock_def,push_env_clock]
-    \\ `x''.clock <= s.clock` by 
+    \\ `x''.clock <= s.clock` by
          (BasicProvers.EVERY_CASE_TAC>>fs[fetch "-" "word_state_component_equality"]>>
-         `F` by DECIDE_TAC)
-    \\ fs[]
-    \\ TRY (`x''.clock = r'''''.clock` by 
+         `F` by DECIDE_TAC) \\ fs[]
+    \\ TRY (`x''.clock = r'''''.clock` by
        (BasicProvers.EVERY_CASE_TAC>>fs[fetch "-" "word_state_component_equality"]))
-    \\ TRY (`x''.clock = r''''''.clock` by 
+    \\ TRY (`x''.clock = r''''''.clock` by
        (BasicProvers.EVERY_CASE_TAC>>fs[fetch "-" "word_state_component_equality"]))
     \\ `F` by DECIDE_TAC)
-
   val new_def = wEval_def |> CONJUNCTS |> map (fst o dest_eq o concl o SPEC_ALL)
                   |> map (REWR_CONV def THENC SIMP_CONV (srw_ss()) [])
                   |> LIST_CONJ
